\titre{Calcul de sommes}
\theme{séries}
\auteur{}
\organisation{AMSCC}

\texte{ Sachant que $\displaystyle e=\sum_{n\geq 0} \frac{1}{n!}$, déterminer la valeur des sommes suivantes : }
\begin{enumerate}
	\item \question{$\displaystyle \sum_{n\geq0} \frac{n+1}{n!}$}
	\reponse{ On décompose la somme en deux sommes :
		\begin{align*}
			\sum_{n\geq0} \frac{n+1}{n!} &= \sum_{n\geq0} \frac{n}{n!} + \sum_{n\geq0} \frac{1}{n!} \\
			&= \sum_{n\geq1} \frac{1}{(n-1)!} + \sum_{n\geq0} \frac{1}{n!} \\
			&= \sum_{n\geq0} \frac{1}{n!} + \sum_{n\geq0} \frac{1}{n!} \\
			&= 2e
		\end{align*}
	}
	
	\item \question{$\sum_{n\geq0} \frac{n^2-2}{n!}$}
	\reponse{ On décompose la somme en deux sommes :
		\begin{align*}
			\sum_{n\geq0} \frac{n^2-2}{n!} &= \sum_{n\geq0} \frac{n^2}{n!} - 2\sum_{n\geq0} \frac{1}{n!} \\
			&= \sum_{n\geq1} \frac{n}{(n-1)!} - 2\sum_{n\geq0} \frac{1}{n!} \\
			&= \sum_{n\geq1} \frac{n-1+1}{(n-1)!} - 2\sum_{n\geq0} \frac{1}{n!} \\
			&= \sum_{n\geq2} \frac{1}{(n-2)!} + \sum_{n\geq 1} \frac{1}{(n-1)!} - 2\sum_{n\geq0} \frac{1}{n!} \\
			&= \sum_{n\geq0} \frac{1}{n!} + \sum_{n\geq 0} \frac{1}{n!} - 2\sum_{n\geq0} \frac{1}{n!} \\
			&= 0
		\end{align*}
	}
	
	\item \question{$\sum_{n\geq0} \frac{n^3}{n!}$}
	\reponse{ On simplifie :
		\begin{align*}
			\sum_{n\geq0} \frac{n^3}{n!} &= \sum_{n\geq0} \frac{n^2}{(n-1)!} \\
			&= \sum_{n\geq1} \frac{n(n-1)+n-1+1}{(n-1)!} \\
			&= \sum_{n\geq1} \frac{n(n-1)}{(n-1)!} + \sum_{n\geq1} \frac{n-1}{(n-1)!} + \sum_{n\geq1} \frac{1}{(n-1)!} \\
			&= \sum_{n\geq2} \frac{n}{(n-2)!} + \sum_{n\geq2} \frac{1}{(n-2)!} + \sum_{n\geq1} \frac{1}{(n-1)!} \\
			&= \sum_{n\geq2} \frac{n-2+2}{(n-2)!} + \sum_{n\geq2} \frac{1}{(n-2)!} + \sum_{n\geq1} \frac{1}{(n-1)!} \\
			&= \sum_{n\geq3} \frac{1}{(n-3)!} + \sum_{n\geq2} \frac{2}{(n-2)!} + \sum_{n\geq2} \frac{1}{(n-2)!} + \sum_{n\geq1} \frac{1}{(n-1)!} \\
			&= \sum_{n\geq0} \frac{1}{n!} + 2\sum_{n\geq0} \frac{1}{n!} + \sum_{n\geq0} \frac{1}{n!} + \sum_{n\geq0} \frac{1}{n!} \\
			&= 5e
		\end{align*}
	}
\end{enumerate}
